Still issues with normalization and new btvs

src/PlutusIR/Semantics/TypeSafety/SubstitutionPreservesTyping/AnnotationSubstitution.v
@@ -2,12 +2,25 @@ Require Import PlutusCert.PlutusIR.Semantics.Static.
 Require Import PlutusCert.PlutusIR.Semantics.Dynamic.
 Require Import PlutusCert.PlutusIR.Semantics.TypeSafety.SubstitutionPreservesTyping.TypeSubstitution.
 
+Require Import PlutusCert.PlutusIR.Semantics.TypeSafety.TypeLanguage.StrongNormalisation.
+Require Import PlutusCert.PlutusIR.Semantics.TypeSafety.BaseKindedness.
+(* From PlutusCert Require Import util. *)
+
+From PlutusCert Require Import FreeVars.
+
+Require Import PlutusCert.PlutusIR.Semantics.Static.Theorems.FreeInContext.
+
 Import PlutusNotations.
 
 Require Import PlutusCert.Util.List.
 
+Require Import PlutusCert.Util.
+
 Require Import Lists.List.
 Import ListNotations.
+
+Require Import Coq.Strings.String.
+Local Open Scope string_scope.
 
 Require Import Coq.Logic.FunctionalExtensionality.
 
@@ -44,11 +57,205 @@ Proof with auto.
       rewrite n...
 Qed.
 
+(* By drop_ty_var, X not in Ty.ftv T*)
+Lemma gsubst__drop_ty_var__substituteT Gamma x X U T :
+    Ty.closed U ->
+    lookup x (drop_ty_var X Gamma) = Datatypes.Some T ->
+    lookup x (drop_ty_var X (gsubst X U Gamma)) = Datatypes.Some T.
+Proof with auto.
+  intros Hclosed Hl.
+  unfold drop_ty_var in *.
+  remember ([]) as R.
+  clear HeqR.
+  generalize dependent R.
+  induction Gamma; intros.
+  - simpl in Hl. inversion Hl.
+  - destruct a as [y V].
+    simpl.
+    destruct (in_dec string_dec X (Ty.ftv (substituteT X U V))).
+    + (* X in substT X U V *)
+      destruct (in_dec string_dec X (Ty.ftv V)).
+      * (* X in V *)
+        eapply IHGamma.
+        (* 
+          ADMIT ( *** ):
+          by lookup x (drop_ty_var X (y, V)::Gamma) = Some T,
+          we know lookup x (drop_ty_var' X Gamma [y]) = Some T 
+
+          (* Then we know x <> y*)
+          Then also lookup x (drop_ty_var X Gamma) = Some T
+        *)
+        admit.
+      * (* X not in V *)
+        exfalso.
+        (* ADMIT: X in substT X U V, but U is closed, so X in V. *)
+        admit.
+    + (* X not in substT X U V *)
+      destruct (in_dec string_dec X (Ty.ftv V)).
+      * (* X in V *)
+        assert (x <> y).
+        {
+        (* ADMIT: X in V, then lookup x (drop_ty_var X ((x, V)) should be None as all keys x will be removed)*)
+        admit.
+        }
+        assert (lookup x (drop_ty_var' X Gamma R) = Some T).
+        {
+          (* See ADMIT ( *** ) *) admit.
+        }
+        destruct (in_dec string_dec y R).
+        -- eapply IHGamma; eauto. 
+        -- simpl.
+           (* destr_eqb_eq y x.
+           ++ contradiction.
+           ++ eapply IHGamma; eauto.  *)
+           admit.
+      * (* X not in V *)
+        assert (lookup x (drop_ty_var' X Gamma R) = Some T).
+        {
+          (* See ADMIT ( *** ) *) admit.
+        }
+        destruct (in_dec string_dec y R).
+        -- eapply IHGamma; eauto.
+        -- simpl.
+           assert (x <> y).
+           {
+             (* ADMIT: x <> y, then lookup x (drop_ty_var X ((x, V)) should be None as all keys x will be removed*)
+             admit.
+           }
+           apply String.eqb_neq in H0.
+           rewrite String.eqb_sym in H0.
+           rewrite H0.
+           eapply IHGamma; eauto.
+
+  (* ADMIT: See comments *)
+Admitted.
+
 Lemma gsubst_absorbs_substituteT : forall x X U T Gamma,
     ((x, (substituteT X U T)) :: gsubst X U Gamma) = gsubst X U ((x, T) :: Gamma).
 Proof.
   reflexivity.
 Qed.
+
+Lemma drop_ty_var__gsubst s X U Γ : 
+  s <> X ->
+  Ty.closed U ->
+  drop_ty_var s (gsubst X U Γ) = gsubst X U (drop_ty_var s Γ).
+Proof.
+  intros Hneq Hclosed.
+  unfold drop_ty_var.
+  remember ([]) as R.
+  clear HeqR.
+  generalize dependent R.
+  induction Γ; intros.
+  - simpl.
+    reflexivity.
+  - destruct a as [x T].
+    simpl.
+    destruct (in_dec string_dec s
+      (Ty.ftv
+      (substituteT X U T))).
+    + destruct (in_dec string_dec s (Ty.ftv T)).
+      * eapply IHΓ.
+      * exfalso.
+        (* ADMIT: s in substT X U T, but U is closed, so s in T. *)
+        admit.
+    + 
+      destruct (in_dec string_dec s (Ty.ftv T)).
+      * exfalso.
+        (* ADMIT: s not in substT X U T 
+                  by s <> X, then s not in T *)
+        admit.
+      * destruct (in_dec string_dec x R).
+        -- eapply IHΓ.
+        -- rewrite <- gsubst_absorbs_substituteT.
+           f_equal.
+           eapply IHΓ.
+(* ADMIT: See comments *)    
+Admitted.
+
+(* TODO: lemma name?
+
+I Doubt this is true because of substituteTCA in normalise
+
+
+ *)
+
+Ltac destruct_match :=
+  match goal with
+  | H : (match ?X with _ => _ end = _ ) |- _ => destruct X eqn:?; try discriminate
+  end.
+
+(* Create cases for x = y and x <> y (where we move from (x =? y) = true -> x = y*)
+Ltac destr_eqb_eq x y :=
+  let H := fresh "H" in
+  destruct (x =? y) eqn:H; [apply String.eqb_eq in H; subst | apply String.eqb_neq in H].
+
+(* Richard: Not true, see schrift *)
+Lemma substituteT__normalisation T Tn SubTn X U:
+  normalise T Tn ->
+  normalise (substituteT X U Tn) SubTn ->
+  normalise (substituteT X U T) SubTn.
+Proof.
+  intros Hnorm__T Hnorm__SubTn.
+  generalize dependent Tn.
+  generalize dependent SubTn.
+  induction T; intros.
+  - inversion Hnorm__T; subst.
+    simpl.
+    (destr_eqb_eq X t).
+    + (* X = t *)
+      simpl in Hnorm__SubTn.
+      rewrite eqb_refl in Hnorm__SubTn.
+      assumption.
+    + (* X <> t *)
+      simpl in Hnorm__SubTn.
+      apply eqb_neq in H.
+      rewrite H in Hnorm__SubTn.
+      assumption.
+  - inversion Hnorm__T; subst.
+    simpl.
+    simpl in Hnorm__SubTn.
+    inversion Hnorm__SubTn; subst.
+    constructor; auto.
+    + eapply IHT1; eauto.
+    + eapply IHT2; eauto.
+  - admit.
+  - admit.
+  - admit.
+  - admit.
+  - (* Ty_App *)
+    simpl.
+    inversion Hnorm__T; subst.
+    + (* N_BetaReduce *)
+      simpl.
+      remember H1 as H1'. clear HeqH1'.
+      assert (exists SubT1n, normalise (substituteT X U (Ty_Lam bX K T1n)) (Ty_Lam bX K SubT1n)) as [SubT1n HSubLamN].
+      {
+        admit.
+      }
+      assert (exists SubT2n, normalise (substituteT X U T2n) SubT2n) as [SubT2n HSubT2n].
+      {
+        admit.
+      }
+
+      eapply IHT1 in H1; eauto.
+      econstructor; eauto.
+      (* subT X U T1n ==> SubT1n
+        
+
+        SubCA bX T2n T1n ==> Tn
+
+        Sub X U Tn ==> SubTn
+
+        ADMIT: Not so clear to me yet.
+      *)
+      admit.
+    + (* N_App *)
+      simpl.
+      simpl in Hnorm__SubTn.
+      (* ADMIT: I DONT KNOW *)
+
+Admitted.
 
 (** ** Predicates *)
 Definition P_Term (t : term) :=
@@ -57,6 +264,200 @@ Definition P_Term (t : term) :=
     [] |-* U : K ->
     normalise (substituteT X U T) Tn ->
     Delta ,, (gsubst X U Gamma) |-+ <{ :[X := U] t }> : Tn.
+
+Local Open Scope string_scope.
+Local Open Scope list_scope.
+
+Definition KB := Kind_Base.
+
+Locate ":[".
+
+(* X is free in t *)
+Definition t := TyInst (TyAbs "X0" KB (TyAbs "X" KB (Var "x"))) (Ty_Var "X").
+Definition T := Ty_Forall (fresh "X0" (Ty_Var "X") <{ ℤ }>) KB <{ ℤ }>.
+
+(*
+  IDEA Jacco: rename approach in TyForall?
+*)
+
+
+(*
+  Λ (X0: * ) (Λ (X :: * ) 3) @ X : SubstitueTCA X0 X  (∀ (X :: * ) Int)
+*)
+
+Definition U := Ty_Builtin DefaultUniBool.
+
+(* THe problem is that here U gets substituted in the type immediately,
+so then no ftvs are in the instantiated type anymore, so then no fresh variable
+is gnerated
+*)
+Definition substA_t : term :=
+  <{ :[ "X" := U ] t }>.
+
+Lemma t_wt :
+  (("X", Kind_Base)::nil),, [("x", <{ ℤ }>)] |-+ t : T. 
+Proof.
+  (* unfold t.
+  unfold T.
+  repeat econstructor; eauto.
+  autorewrite with substituteTCA.
+  assert ("X0" <> "X") by admit. (* ADMIT: non-identical strings*)
+  apply eqb_neq in H.
+  rewrite H.
+  assert (existsb (eqb "X") (ftv (Ty_Var "X")) = true) by admit. (* ADMIT: "X" = "X"*)
+  rewrite H0.
+  simpl.
+  assert (Hren_builtin: (rename "X"
+  (fresh "X0" (Ty_Var "X") <{ ℤ }>)
+  <{ ℤ }>) = <{ ℤ }>) by admit. (* ADMIT: no ftvs in TInt to rename *)
+  rewrite Hren_builtin; clear Hren_builtin.
+  autorewrite with substituteTCA.
+  constructor. constructor. *)
+Admitted.
+
+Definition T2 := Ty_Forall "X" KB <{ ℤ }>.
+
+Lemma substA_t_wt :
+  [] ,, [("x", <{ ℤ }>)] |-+ substA_t : T2.
+Proof.
+  unfold substA_t.
+  unfold T.
+  simpl.
+  repeat econstructor; eauto.
+  autorewrite with substituteTCA.
+  assert ("X0" <> "X") by admit. (* ADMIT: non-identical strings*)
+  apply eqb_neq in H.
+  (* rewrite H.
+  assert (existsb (eqb "X") (ftv (U)) = false) by admit. (* no ftv in Bool *)
+  unfold U in H0.
+  rewrite H0.
+  unfold T2.
+  constructor.
+  constructor. *)
+Admitted.
+
+(* We also know U is closed, but do not need it yet *)
+Lemma commute_substituteT :
+  forall X U V T,
+    substituteT X U (substituteT X V T) = substituteT X (substituteT X U V) T.
+Proof.
+  intros X U V T.
+  induction T.
+  - simpl.
+    destr_eqb_eq X t0; auto.
+    simpl.
+    apply eqb_neq in H; rewrite H; auto.
+  - simpl.
+    f_equal.
+    apply IHT1; auto.
+    apply IHT2; auto.
+  - simpl.
+    f_equal.
+    apply IHT1; auto.
+    apply IHT2; auto.
+  - simpl.
+    destr_eqb_eq X b; auto.
+    simpl.
+    rewrite String.eqb_refl; auto.
+    simpl.
+    apply eqb_neq in H; rewrite H; auto.
+    f_equal.
+    apply IHT; auto.
+  - simpl. reflexivity.
+  - simpl.
+    destr_eqb_eq X b; auto.
+    simpl.
+    rewrite String.eqb_refl; auto.
+    simpl.
+    apply eqb_neq in H; rewrite H; auto.
+    f_equal.
+    apply IHT; auto.
+  - simpl.
+    f_equal.
+    apply IHT1; auto.
+    apply IHT2; auto.
+Admitted.
+
+Lemma substituteT_vacuous_closed X U T :
+    Ty.closed T ->
+    substituteT X U T = T.
+Admitted.
+
+(* NOTE: commute_sub_naive *)
+Lemma commute_substituteT_2 :
+  forall X X0 U V T,
+    X <> X0 -> (* TODO: necessary? Maybe without it this implies commute_substituteT *)
+    Ty.closed U ->
+    (* TODO: Required: binders in T are not free in V? *)
+    substituteT X0 (substituteT X U V) (substituteT X U T) = 
+      substituteT X U (substituteT X0 V T).
+Proof.
+  intros X X0 U V T Hneq Uclosed.
+  induction T.
+  - simpl.
+    destr_eqb_eq X t0; auto.
+    + simpl.
+      apply eqb_neq in Hneq.
+      rewrite String.eqb_sym in Hneq; rewrite Hneq.
+      simpl.
+      rewrite String.eqb_refl; auto.
+      apply substituteT_vacuous_closed; auto.
+    + simpl.
+      destr_eqb_eq X0 t0; auto.
+      simpl.
+      apply eqb_neq in H; rewrite H. reflexivity.
+  - simpl.
+    f_equal.
+    apply IHT1; auto.
+    apply IHT2; auto.
+  - simpl.
+    f_equal.
+    apply IHT1; auto.
+    apply IHT2; auto.
+  - simpl.
+    destr_eqb_eq X b; destr_eqb_eq X0 b; auto.
+    + contradiction Hneq. reflexivity.
+    + simpl.
+      rewrite String.eqb_refl; auto.
+      apply eqb_neq in H; rewrite H.
+      f_equal.
+      (* What if b in V? *)
+      admit.
+    + simpl.
+      rewrite String.eqb_refl; auto.
+      apply eqb_neq in H; rewrite H.
+      f_equal.
+    + simpl.
+      apply eqb_neq in H; rewrite H.
+      apply eqb_neq in H0; rewrite H0.
+      rewrite IHT.
+      reflexivity.
+  - simpl. reflexivity.
+  - (* Ty_Lam *)
+    simpl.
+    destr_eqb_eq X b; destr_eqb_eq X0 b; auto.
+    + contradiction Hneq. reflexivity.
+    + simpl.
+      rewrite String.eqb_refl; auto.
+      apply eqb_neq in H; rewrite H.
+      f_equal.
+      (* What if b in V? *)
+      admit.
+    + simpl.
+      rewrite String.eqb_refl; auto.
+      apply eqb_neq in H; rewrite H.
+      f_equal.
+    + simpl.
+      apply eqb_neq in H; rewrite H.
+      apply eqb_neq in H0; rewrite H0.
+      rewrite IHT.
+      reflexivity.
+  - (* Ty_App *)
+    simpl.
+    f_equal.
+    apply IHT1; auto.
+    apply IHT2; auto.
+Admitted.
 
 Definition P_Binding (b : binding) : Prop :=
   forall Delta Gamma rec X K U,
@@ -69,6 +470,7 @@ Definition P_Binding (b : binding) : Prop :=
   P_Binding
   : core.
 
+
 Theorem substA_preserves_typing :
   forall t, P_Term t.
 Proof with (eauto using substituteT_preserves_kinding with typing).
@@ -77,7 +479,468 @@ Proof with (eauto using substituteT_preserves_kinding with typing).
   all: unfold P_Term.
   all: try (intros Delta Gamma X K U T Tn Htyp__t Hkind__U Hnorm__Tn).
   all: unfold P_Binding.
-  all: try (intros Delta Gamma X K U Htyp__b Hkind__U).
+  all: try (intros Delta Gamma rec X K U Htyp__b Hkind__U).
   all: try (inversion Htyp__t; subst).
+  - (* Let (NonRec) *)
+    simpl.
+    econstructor; eauto.
+    + admit.
+    + (* probably *) admit.
+    + 
+       destruct (existsb (eqb X) (btvbs bs)).
+      * (* X in btvbs bs *)
+        simpl.
+        (* Everything gets renamed accordingly, should hold?*)
+        admit.
+      * (* X not in btvbs bs *)
+        assert (@substA_bnr' substA_b X U bs = bs).
+        {
+          (* ADMIT: I think this is true, but not sure yet *)
+          admit.
+        }
+        rewrite H1.
+        (* hmm. Then X should also not be appearing in Gamma *)
+        unfold P_Term in H0.
+        (* eapply H0. TODO: Cannot apply it because bsGn is in front of the gsubst. we can probably drag it inside *)
+        admit.
+    + (* I think the key here is that there is no longer an X in substituteT X U T. *)
+      admit.
+  - (* Let Rec *)
+    admit.
+  - (* Var *)
+    simpl.
+    econstructor.
+    + eapply gsubst__substituteT; eauto.
+    + eapply substituteT_preserves_kinding; eauto.
+    + eapply substituteT__normalisation; eauto.
+  - (* TyAbs *)
+    simpl.
+    destr_eqb_eq X s.
+    + (* X = s *)
+      simpl substituteT in Hnorm__Tn.
+      destr_eqb_eq s Y.
+      * (* Y = s = X *)
+        assert (Hsub2: substituteT Y (Ty_Var Y) Tn0 = Tn0) by admit.
+        inversion Hnorm__Tn; subst.
+        assert (Hsub3: substituteT Y (Ty_Var Y) T0n = T0n) by admit.
+        rewrite <- Hsub3.
+        apply T_TyAbs; auto.
+        -- admit.
+        -- admit.
+        -- 
+          (* Y not in btv T0n??? But normalise could create them!!! No, because Tn0 is already
+            normal and normal stable *)
+          admit.
+      * (* Y <> s   and X = s*)
+        inversion Hnorm__Tn; subst.
+        assert (substituteT s U (substituteT s (Ty_Var Y) Tn0) = substituteT s (Ty_Var Y) Tn0) by admit. (* vac sub*)
+        (* Also sub t Y Tn0 is normal, by Y fresh and Tn0 normal*)
+        rewrite H1 in H6.
+        assert (T0n = substituteT s (Ty_Var Y) Tn0) by admit.
+        rewrite H2.
+        apply T_TyAbs; auto.
+        -- (* Some drop_ty_var arguments *) admit.
+    + destr_eqb_eq s Y.
+      * (* s = Y   and X <> s *) 
+        simpl in Hnorm__Tn.
+        rewrite <- String.eqb_neq in H0.
+        rewrite H0 in Hnorm__Tn.
+        inversion Hnorm__Tn; subst.
+        assert (T0n = substituteT Y (Ty_Var Y) T0n) by admit.
+        rewrite H1.
+        eapply T_TyAbs; auto.
+        -- admit.
+        -- (* no ftvs created, U closed, etc.*)
+           admit.
+        -- (* ADMIT: We assume now that normalise does not create new ftvs (but it can)!*)
+           admit.
+      * (* s <> Y and X <> s*)
+
+        (* X = Y, then we have no substituteT in types. 
+           On term level?
+        *)
+        simpl in Hnorm__Tn.
+        destr_eqb_eq X Y.
+        -- (* X = Y *)
+           unfold P_Term in H.
+           inversion Hnorm__Tn; subst.
+           assert (substituteT s (Ty_Var Y) Tn0 = T0n) by admit. (* ADMIT: Not true, assume normality = equality*)
+           rewrite <- H2.
+           constructor; auto.
+           assert (drop_ty_var Y (gsubst Y U Gamma) = gsubst Y U Gamma).
+           {
+             (* ADMIT: I think this is true, but not sure yet *)
+             admit.
+           }
+           rewrite H3.
+           rewrite drop_ty_var__gsubst; auto.
+           {
+            eapply H with (T := Tn0) (K := K); eauto.
+            - (* By drop_ty_var inclusion? and weakening?
+                drop_ty_var Y Gamma included in Gamma
+
+                Then drop s (drop Y Gamma) included in Gamma
+            *)
+            
+            
+              (* ADMIT: Weakening permute *) admit.
+            - (* Y not in Tn0, so vacuous subst, so yes *) admit.
+           }
+           ++ (* U closed *) admit.
+
+
+
+        -- (* s, X, Y disctinct *)
+           inversion Hnorm__Tn; subst.
+           (* Let's assume for now that it is already normal: *)
+           assert (substituteT X U (substituteT s (Ty_Var Y) Tn0) = substituteT s (Ty_Var Y) (substituteT X U Tn0)) by admit.
+           rewrite H3 in H10.
+           assert (T0n = substituteT s (Ty_Var Y) (substituteT X U Tn0)) by admit.
+           rewrite H4.
+           constructor; auto.
+           ++ unfold P_Term in H. clear H3 H4.
+              rewrite drop_ty_var__gsubst; auto.
+              rewrite drop_ty_var__gsubst; auto.
+              eapply H with (T := Tn0) (K := K); eauto.
+              ** (* ADMIT: Weakening permute *) admit.
+              ** (* ADMIT: We forget about normalisation for now *) admit.
+              ** (* U closed*) admit.
+              ** (* U closed *) admit.
+          ++ (* normalise does not create new ftvs and U clsoed *)admit.
+          ++ (* ADMIT: We assume now that normalise does not create new btvs (but it can)!*)
+             admit.
+
+  - (* LamAbs *)
+    simpl.
+    simpl substituteT in Hnorm__Tn.
+    inversion Hnorm__Tn; subst.
+    constructor; auto.
+    * eapply substituteT_preserves_kinding; eauto.
+    * eapply substituteT__normalisation; eauto.
+    * assert ((s, substituteT X U T1n) :: gsubst X U Gamma = gsubst X U ((s, T1n) :: Gamma)).
+      {
+        rewrite gsubst_absorbs_substituteT; auto.
+      }
+      assert (Hgsubst_not_normal: 
+        (s, (substituteT X U T1n)) :: (gsubst X U Gamma) = 
+          (s, T1n0) :: gsubst X U Gamma).
+      {
+      (* ADMIT: substituteT X U T1n may not be normal, 
+          how to reconcile? Must gsubst also normalise? 
+          Maybe find counterexample tomorrow.
+
+          Or does typing context not have to be normal?
+          Something like, if it is well_typed for T in gamma,
+          then it is well_typed for Tn in gamma.
+          *)
+          admit.
+      }
+      rewrite <- Hgsubst_not_normal.
+      unfold P_Term in H.
+      rewrite H0.
+      eapply H; eauto.
+  - (* Apply *)
+    simpl.
+    assert (Delta |-* (substituteT X U T1n) : Kind_Base).
+    {
+      eapply substituteT_preserves_kinding; eauto.
+      eapply has_type__basekinded; eauto.
+    }
+    eapply strong_normalisation in H1 as [subT1n HsubT1n].
+      
+    econstructor.
+    + 
+      eapply H; eauto.
+      simpl substituteT.
+      constructor; eauto.
+    + eapply H0; eauto.
+  - (* Constant *)
+    simpl.
+    inversion Hnorm__Tn; subst.
+    constructor.
+  - (* Builtin *)
+    simpl.
+    (* Probably: 
+    ADMIT:
+      closed (lookupBuildtinTy d)
+        Then closed T, but also lookupBuiltinTy d = T.
+        Then substituteT X U T = T.
+        Then normalise T Tn => T = Tn.
+     *)
+     assert (T = Tn) by admit.
+     subst.
+     econstructor; eauto.
+  - (* TyInst *)
+    simpl.
+    unfold P_Term in H.
+    destr_eqb_eq X X0.
+    + (* X = X0 *)
+      assert (exists T1nn, normalise T1n T1nn) as [T1nn HT1nn].
+      {
+        eapply strong_normalisation; eauto.
+        apply has_type__basekinded in H2.
+        inversion H2; subst.
+        eauto.
+      } 
+      assert (exists subt0, normalise (substituteT X0 U t1) subt0) as [subt0 Hsubt0].
+        {
+          eapply strong_normalisation; eauto.
+          apply has_type__basekinded in H2.
+          inversion H2; subst.
+          eauto.
+          eapply substituteT_preserves_kinding; eauto.
+      }
+      
+      econstructor.
+      * eapply H; auto.
+        simpl substituteT.
+        -- eauto.
+        -- assumption.
+        -- simpl substituteT.
+           rewrite eqb_refl.
+           constructor; eauto.
+      * eapply substituteT_preserves_kinding; eauto.
+      * eauto.
+      * (*
+        We know:   normalise (substituteT X0 U T) Tn
+         and       normalise (substituteTCA X0 T2n T1n) T.
+
+         Hence     normalise (substituteT X0 U (subsituteTCA X0 T2n T1n)) Tn.      
+
+         Also   normalise T1n T1nn
+          Hence     normalise (substituteT X0 U (subsituteTCA X0 T2n T1nn)) Tn.
+
+          So let us simplify the argument by (wrongly) equating normal stuff
+        *)
+        assert (T1nn = T1n) by admit. clear HT1nn. subst.
+        assert (T2n = t1) by admit. clear H6. subst.
+        assert (subt0 = substituteT X0 U t1) by admit. clear Hsubt0. subst.
+        assert (Tn = substituteT X0 U T) by admit. clear Hnorm__Tn. subst.
+        assert (T = (substituteTCA X0 t1 T1n)) by admit. clear H8. subst.
+        (* Is that true? I fear alpha equivalence.
+          Create some examples.
+          It is not.
+        *)
+
+        assert (normalise
+          (substituteTCA X0 (substituteT X0 U t1) T1n)
+          (substituteT X0 U (substituteTCA X0 t1 T1n))
+            = normalise
+          (substituteT X0 (substituteT X0 U t1) T1n)
+          (substituteT X0 U (substituteT X0 t1 T1n))
+        ).
+        {        (* 
+          ADMIT: What if we have substituteT instead of substituteTCA, is it true then?
+          Yes.
+        *)
+          admit.
+        }
+        rewrite H0.
+        erewrite commute_substituteT.
+        (* ADMIT: They are identical, but the latter does not need to be normal yet. I think that is
+            solved by not doing all thsoe admits above
+          *)
+
+
+        admit.
+    + (* X <> X0 *)
+      assert (exists subT1n, normalise (substituteT X U t1) subT1n) as [subT1n HsubT1n].
+        {
+          eapply strong_normalisation; eauto.
+          apply has_type__basekinded in H2.
+          inversion H2; subst.
+          eauto.
+          eapply substituteT_preserves_kinding; eauto.
+      }
+
+      assert (exists SubT1nn, normalise (substituteT X U T1n) SubT1nn) as [SubT1nn HT1nn].
+      {
+        eapply strong_normalisation; eauto.
+        apply has_type__basekinded in H2.
+        inversion H2; subst.
+        eauto.
+        eapply substituteT_preserves_kinding; eauto.
+        eapply Kinding.weakening; eauto.
+        admit.
+        (* apply inclusion_swap; eauto. *)
+      } 
+
+      econstructor.
+      * eapply H; eauto.
+        simpl substituteT.
+        apply eqb_neq in H0.
+        rewrite H0.
+        constructor; eauto.
+      * eapply substituteT_preserves_kinding; eauto.
+      * eauto.
+      * (* ADMIT: Just like above for now equating all the normal stuff: *)
+        assert (t1 = T2n) by admit; subst.
+        assert (substituteT X U T2n = subT1n) by admit; subst.
+        assert (substituteT X U T1n = SubT1nn) by admit; subst.
+        assert (substituteTCA X0 T2n T1n = T) by admit; subst.
+        clear HT1nn HsubT1n H8 H6.
+        assert (substituteT X U (substituteTCA X0 T2n T1n) = Tn) by admit; subst.
+        clear Hnorm__Tn.
+
+        (* Aha, so it is not the same as above, X <> X0 *)
+
+        (* We want to call commute_substituteT_2 with V := T2n, and with T := T1n
+            And we need: btv in T not free in V
+              That is like exactly NC T [? -> V] from the alpha stuff
+            
+          If we change the TyInst rule as I suggested to Jacco:
+          typechecking the rhs of TyInst with smaller Delta,
+            then we have this assumption I think
+        *)
+         admit.
+  - (* Error *)
+    (* ADMIT: Probably we do not need to do this for Error since we are not doing preservation for non-error*)
+    admit.
+  - (* IWrap *)
+    simpl.
+    simpl in Hnorm__Tn.
+    inversion Hnorm__Tn; subst.
+    assert (exists subTXUT0n, normalise (substituteT X U T0n) subTXUT0n) as [subTXUT0n HsubTXUT0n].
+    {
+      eapply strong_normalisation; eauto.
+      admit.
+    }
+
+    eapply T_IWrap with (T0n := subTXUT0n).
+    + eapply substituteT_preserves_kinding; eauto.
+    + eapply substituteT__normalisation; eauto.
+    + eapply substituteT_preserves_kinding; eauto.
+    + eapply substituteT__normalisation; eauto.
+    + (* ADMIT: not sure yet, but probably some more convoluted case of substituteT__normalisation 
+      *)
+      admit.
+    + eapply H; eauto.
+  - (* Unwrap *)
+    assert (exists sub_XU_Tn0, normalise (substituteT X U Tn0) sub_XU_Tn0) as [sub_XU_Tn0 Hsub_XU_Tn0].
+    {
+      eapply strong_normalisation; eauto.
+      eapply substituteT_preserves_kinding; eauto.
+    }
+    remember H1 as H1'. clear HeqH1'.
+    eapply has_type__basekinded in H1'; eauto.
+    inversion H1'; subst.
+    assert (exists sub_XU_Fn, normalise (substituteT X U Fn) sub_XU_Fn) as [sub_XU_Fn Hsub_XU_Fn].
+    {
+      eapply strong_normalisation; eauto.
+      eapply substituteT_preserves_kinding; eauto.
+    }
+    simpl.
+    eapply T_Unwrap.
+    + eapply H; eauto.
+      simpl.
+      constructor; eauto.
+    + admit.
+    + (* ADMIT: Not sure yet *)
+    admit.
+  - (* TermBind *)
+    simpl.
+    destruct v.
+    inversion Htyp__b; subst.
+    assert (exists sub_XU_Tn, normalise (substituteT X U t1) sub_XU_Tn) as [sub_XU_Tn H_sub_XU_Tn].
+    {
+      eapply strong_normalisation; eauto.
+      eapply substituteT_preserves_kinding; eauto.
+    }
+    econstructor.
+    + eapply substituteT_preserves_kinding; eauto.
+    + eauto.
+    + eapply H; eauto.
+      (* ADMIT: 
+         
+         norm t1 Tn
+         norm (sub X U t1) sub_XU_Tn
+         =>
+         norm (sub X U Tn) sub_XU_Tn 
+      *)
+      admit.
+  - (* TypeBind *)
+    simpl.
+    inversion Htyp__b; subst.
+    econstructor.
+    eapply substituteT_preserves_kinding; eauto.
+  - (* DatatypeBind *)
+    simpl.
+    destruct dtd.
+    inversion Htyp__b; subst.
+    inversion H0; subst; clear H0.
+    simpl in *.
+    destruct rec.
+    + (* NonRec *)
+
+      (* ADMIT: No time to finish this*)
+      admit.
+    + (* Rec *)
+      econstructor; eauto.
+      * admit.
+      * intros.
+        simpl.
+        (* [X := U]cs cs must contain Vardecls*)
+        induction cs; [inversion H|].
+        simpl in H.
+        destruct a.
+        destruct H.
+        -- subst.
+           simpl.
+           econstructor.
+           3: eauto.
+           ++ admit.
+           ++ admit.
+        -- eapply IHcs; eauto.
+           ++ (* uhm*) admit.
+           ++ (* NODUP smaller *) admit.
+           ++ (* hmmm, not getting closer *)
+            admit.
+      * simpl.
+        (* ADMIT: How can this be true? We must know XK already in Delta?
+          This seems to be problematic in the special case where the variable we are substituting (X)
+          is equal to the datatype name.
+
+          Probably indeed the datatype name should not be renamed (it is like a tyabs binder), but
+          how to reconcile XK = X?
+
+          We should know from bindings_well_formed_rec that X is already in Delta
+          But even then, this creates weird things, for instance if K is of a different kind then what
+          it has in Delta.
+        *)
+        admit.
+    
+  
 (* ADMIT: I had no time to finish this. Should follow from uniqueness property, amongst others. *)
 Admitted.
+
+Corollary substA_preserves_typing__Term : 
+  forall Delta Gamma X K U t T Tn,
+    ((X, K) :: Delta) ,, Gamma |-+ t : T ->
+    [] |-* U : K ->
+    normalise (substituteT X U T) Tn ->
+    Delta ,, (gsubst X U Gamma) |-+ <{ :[X := U] t }> : Tn.
+Proof.
+  intros.
+  eapply substA_preserves_typing; eauto.
+Qed.
+
+Corollary substA_preserves_typing__Term__value : 
+  forall X K U t T Tn,
+    ((X, K) :: nil) ,, nil |-+ t : T ->
+    [] |-* U : K -> (* 
+    
+      So.. no capture?
+      No free vars in U, hence a binder in T cannot capture that
+
+    *)
+    normalise (substituteT X U T) Tn ->
+    nil ,, nil |-+ <{ :[X := U] t }> : Tn.
+Proof.
+  intros.
+  assert (nil ,, (gsubst X U nil) |-+ <{ :[X := U] t }> : Tn).
+  {
+    eapply substA_preserves_typing__Term; eauto.
+  }
+  simpl in H2.
+  auto.
+Qed.
