src/PlutusIR/Semantics/TypeSafety/TypeLanguage/Preservation.v
@@ -1,6 +1,5 @@
 Require Import PlutusCert.PlutusIR.Semantics.Static.
 Require Import PlutusCert.PlutusIR.Semantics.Dynamic.
-Require Import PlutusCert.PlutusIR.Semantics.TypeSafety.SubstitutionPreservesTyping.
 
 Theorem preservation : forall Delta T K Tn,
     Delta |-* T : K ->
